import Relation.Binary.PropositionalEquality as Eq
open Eq using (_â‰¡_; refl; cong; sym)

-- Negation
data âŠ¥ : Set where
  -- empty

Â¬_ : Set â†’ Set
Â¬ A = (A â†’ âŠ¥)

âŠ¥-elim : {A : Set} â†’ âŠ¥ â†’ A
âŠ¥-elim ()

-- First, we define the syntax of our language as in the book
data Term : Set where
  TmTrue   : Term
  TmFalse  : Term
  TmIf     : Term â†’ Term â†’ Term â†’ Term
  TmZero   : Term
  TmSucc   : Term â†’ Term
  TmPred   : Term â†’ Term
  TmIsZero : Term â†’ Term

-- We declare which of the terms are values
data NumericalValue : Term â†’ Set where
  zero  : NumericalValue TmZero
  sucNv : âˆ€ {t : Term} â†’ NumericalValue t â†’ NumericalValue (TmSucc t)

data Value : Term â†’ Set where
  true       : Value TmTrue
  false      : Value TmFalse
  numericVal : âˆ€ {t : Term} â†’ NumericalValue t â†’ Value t

-- Now we can translate the operational semantics into a predicate
data _â†ª_ : Term â†’ Term â†’ Set where
  E-IfTrue     : âˆ€ {tâ‚‚ tâ‚ƒ : Term} â†’ TmIf TmTrue tâ‚‚ tâ‚ƒ â†ª tâ‚‚
  E-IfFalse    : âˆ€ {tâ‚‚ tâ‚ƒ : Term} â†’ TmIf TmFalse tâ‚‚ tâ‚ƒ â†ª tâ‚ƒ
  E-PredZero   : TmPred TmZero â†ª TmZero
  E-PreddSucc  : âˆ€ {t : Term} â†’ NumericalValue t â†’ TmPred (TmSucc t) â†ª t 
  E-Pred       : âˆ€ {tâ‚ tâ‚'} â†’ tâ‚ â†ª tâ‚' â†’ TmPred tâ‚ â†ª TmPred tâ‚'
  E-If         : âˆ€ {tâ‚ tâ‚' tâ‚‚ tâ‚ƒ : Term} â†’ tâ‚ â†ª tâ‚' â†’ TmIf tâ‚ tâ‚‚ tâ‚ƒ â†ª TmIf tâ‚' tâ‚‚ tâ‚ƒ
  E-Succ       : âˆ€ {tâ‚ tâ‚' : Term} â†’ tâ‚ â†ª tâ‚' â†’ TmSucc tâ‚ â†ª TmSucc tâ‚'
  E-IsZero     : âˆ€ {tâ‚ tâ‚' : Term} â†’ tâ‚ â†ª tâ‚' â†’ TmIsZero tâ‚ â†ª TmIsZero tâ‚'
  E-IsZeroSucc : âˆ€ {tâ‚ : Term} â†’ NumericalValue tâ‚ â†’ TmIsZero (TmSucc tâ‚) â†ª TmFalse
  E-IsZeroZero : TmIsZero TmZero â†ª TmTrue
  
-- Now we can for example prove for example, the determinacy property from the book:
lemma : âˆ€ {t t' : Term} â†’ t â†ª t' â†’ Â¬ Value t
lemma (E-Succ tâ†ªt') (numericVal (sucNv x)) = lemma tâ†ªt' (numericVal x)

â†ª-determinacy : âˆ€ {t t' t'' : Term} â†’ t â†ª t' â†’ t â†ª t'' â†’ t' â‰¡ t''
â†ª-determinacy E-IfTrue E-IfTrue = refl
â†ª-determinacy E-IfFalse E-IfFalse = refl
â†ª-determinacy E-PredZero E-PredZero = refl
â†ª-determinacy (E-PreddSucc x) (E-PreddSucc xâ‚) = refl
â†ª-determinacy (E-PreddSucc x) (E-Pred tâ†ªt'') = âŠ¥-elim (lemma tâ†ªt'' (numericVal (sucNv x)))
â†ª-determinacy (E-Pred tâ†ªt') (E-PreddSucc x) = âŠ¥-elim (lemma tâ†ªt' (numericVal (sucNv x)))
â†ª-determinacy (E-Pred tâ†ªt') (E-Pred tâ†ªt'') = cong TmPred (â†ª-determinacy tâ†ªt' tâ†ªt'')
â†ª-determinacy (E-If {tâ‚} {tâ‚'} {tâ‚‚} {tâ‚ƒ} tâ†ªt') (E-If {tâ‚} {tâ‚''} {tâ‚‚} {tâ‚ƒ} tâ†ªt'') = cong (Î» x â†’ TmIf x tâ‚‚ tâ‚ƒ) (â†ª-determinacy tâ†ªt' tâ†ªt'')
â†ª-determinacy (E-Succ tâ†ªt') (E-Succ tâ†ªt'') = cong TmSucc (â†ª-determinacy tâ†ªt' tâ†ªt'')
â†ª-determinacy (E-IsZero tâ†ªt') (E-IsZero tâ†ªt'') = cong TmIsZero (â†ª-determinacy tâ†ªt' tâ†ªt'')
â†ª-determinacy (E-IsZero (E-Succ ())) (E-IsZeroSucc zero)
â†ª-determinacy (E-IsZero (E-Succ (E-Succ tâ†ªt'))) (E-IsZeroSucc (sucNv x)) = âŠ¥-elim (lemma tâ†ªt' (numericVal x))
â†ª-determinacy (E-IsZeroSucc zero) (E-IsZero (E-Succ ()))
â†ª-determinacy (E-IsZeroSucc (sucNv x)) (E-IsZero (E-Succ (E-Succ tâ†ªt''))) = âŠ¥-elim (lemma tâ†ªt'' (numericVal x))
â†ª-determinacy (E-IsZeroSucc x) (E-IsZeroSucc xâ‚) = refl
â†ª-determinacy E-IsZeroZero E-IsZeroZero = refl

-- We can also evaluate terms by writing a function for the single-step evaluation rules
-- For this, we define values a bit more simple in terms of booleans as follows
data ğ”¹ : Set where
  false : ğ”¹
  true  : ğ”¹

isNumericValue : Term â†’ ğ”¹
isNumericValue TmZero = true
isNumericValue (TmSucc t) = isNumericValue t
isNumericValue _ = false

isValue : Term â†’ ğ”¹
isValue TmTrue = true
isValue TmFalse = true
isValue t = isNumericValue t

-- We also define an option type, equivalent to Haskell's Maybe
-- to capsule the case when we enter a normal form
data Option (A : Set) : Set where
  some    : A â†’ Option A
  nothing : Option A

eval-helper : Term â†’ Option Term

eval : Term â†’ Option Term
eval (TmIf TmTrue tâ‚‚ tâ‚ƒ)  = some tâ‚‚
eval (TmIf TmFalse tâ‚‚ tâ‚ƒ) = some tâ‚ƒ
eval (TmIf tâ‚ tâ‚‚ tâ‚ƒ) with eval tâ‚
... | some t  = some (TmIf t tâ‚‚ tâ‚ƒ)
... | nothing = nothing
eval (TmPred TmZero) = some TmZero
eval (TmPred (TmSucc t)) with isNumericValue t
... | true  = some t 
... | false = eval-helper (TmPred (TmSucc t))
eval (TmSucc tâ‚) with eval tâ‚
... | some t  = some (TmSucc t)
... | nothing = nothing
eval (TmIsZero TmZero) = some TmTrue
eval (TmIsZero (TmSucc t)) with isNumericValue t
... | true  = some TmFalse
... | false = eval-helper (TmIsZero (TmSucc t))
eval t = eval-helper t

eval-helper (TmPred t) with eval t
... | some tâ‚ = some (TmPred tâ‚)
... | nothing = nothing
eval-helper (TmIsZero t) with eval t
... | some tâ‚ = some (TmIsZero tâ‚)
... | nothing = nothing
eval-helper _ = nothing
